refactor: flesh out the axioms a little more

LeanSAT/AIG/RelabelNat.lean
@@ -6,9 +6,11 @@ variable {α : Type} [BEq α] [Hashable α]
 
 namespace AIG
 
+namespace RelabelNat
+
 inductive State.Inv1 : Nat → HashMap α Nat → Prop where
-| empty : State.Inv1 0 {}
-| insert (hinv : State.Inv1 n map) (hfind : map.find? x = none) : State.Inv1 (n + 1) (map.insert x n)
+| empty : Inv1 0 {}
+| insert (hinv : Inv1 n map) (hfind : map.find? x = none) : Inv1 (n + 1) (map.insert x n)
 
 /--
 Proof sketch for this axiom once we have more `HashMap` theory:
@@ -28,34 +30,101 @@ Proof sketch for this axiom once we have more `HashMap` theory:
 axiom State.Inv1.property {n m : Nat} (x y : α) (map : HashMap α Nat) (hinv : State.Inv1 n map)
     (hfound1 : map.find? x = some m) (hfound2 : map.find? y = some m) : x = y
 
-structure State (α : Type) [BEq α] [Hashable α] where
+inductive State.Inv2 (decls : Array (Decl α)) : Nat → HashMap α Nat → Prop where
+| empty : Inv2 decls 0 {}
+| newAtom (hinv : Inv2 decls idx map) (hlt : idx < decls.size) (hatom : decls[idx] = .atom a)
+  (hmap : map.find? a = none)
+  : Inv2 decls (idx + 1) (map.insert a val)
+| oldAtom (hinv : Inv2 decls idx map) (hlt : idx < decls.size) (hatom : decls[idx] = .atom a)
+  (hmap : map.find? a = some n)
+  : Inv2 decls (idx + 1) map
+| const (hinv : Inv2 decls idx map) (hlt : idx < decls.size) (hatom : decls[idx] = .const b)
+  : Inv2 decls (idx + 1) map
+| gate (hinv : Inv2 decls idx map) (hlt : idx < decls.size) (hatom : decls[idx] = .gate l r li ri)
+  : Inv2 decls (idx + 1) map
+
+theorem State.Inv2.upper_lt_size {decls : Array (Decl α)} (hinv : Inv2 decls upper map)
+    : upper ≤ decls.size := by
+  cases hinv <;> omega
+
+axiom State.Inv2.property (decls : Array (Decl α)) (idx upper : Nat) (map : HashMap α Nat)
+    (hinv : Inv2 decls upper map)
+    : ∀ (hidx : idx < upper), ∀ (a : α),
+        decls[idx]'(by have := upper_lt_size hinv; omega) = .atom a
+          → ∃ n, map.find? a = some n
+
+structure State (α : Type) [BEq α] [Hashable α] (decls : Array (Decl α)) (idx : Nat) where
   max : Nat
   map : HashMap α Nat
   inv1 : State.Inv1 max map
+  inv2 : State.Inv2 decls idx map
 
-def State.empty : State α :=
-  { max := 0, map := {}, inv1 := State.Inv1.empty }
+def State.empty {decls : Array (Decl α)} : State α decls 0 :=
+  { max := 0, map := {}, inv1 := State.Inv1.empty, inv2 := State.Inv2.empty }
 
-def State.addVar (state : State α) (x : α) : State α :=
-  match h:state.map.find? x with
-  | some _ => state
+def State.addVar {decls : Array (Decl α)} (state : State α decls idx) (a : α)
+    (h : decls[idx]'sorry = .atom a)
+    : State α decls (idx + 1) :=
+  match hmap:state.map.find? a with
+  | some _ =>
+    { state with
+        inv2 := by
+          apply Inv2.oldAtom
+          . exact state.inv2
+          . assumption
+          . assumption
+    }
   | none =>
     {
       max := state.max + 1
-      map := state.map.insert x state.max
+      map := state.map.insert a state.max
       inv1 := by
         apply State.Inv1.insert
         . exact state.inv1
-        . exact h
+        . assumption
+      inv2 := by
+        apply Inv2.newAtom
+        . exact state.inv2
+        . assumption
+        . assumption
     }
 
-def State.addDecl (state : State α) (decl : Decl α) : State α :=
-  match decl with
-  | .atom x => state.addVar x
-  | _ => state
+def State.addConst {decls : Array (Decl α)} (state : State α decls idx) (b : Bool)
+    (h : decls[idx]'sorry = .const b)
+    : State α decls (idx + 1) :=
+  { state with
+      inv2 := by
+        apply Inv2.const
+        . exact state.inv2
+        . assumption
+  }
 
-def State.ofAIGAux (aig : AIG α) : State α :=
-  aig.decls.foldl (init := State.empty) State.addDecl
+def State.addGate {decls : Array (Decl α)} (state : State α decls idx) (lhs rhs : Nat)
+    (linv rinv : Bool) (h : decls[idx]'sorry = .gate lhs rhs linv rinv)
+    : State α decls (idx + 1) :=
+  { state with
+      inv2 := by
+        apply Inv2.gate
+        . exact state.inv2
+        . assumption
+  }
+
+def State.ofAIGAux (aig : AIG α) : State α aig.decls aig.decls.size :=
+  go aig.decls 0 State.empty
+where
+  go (decls : Array (Decl α)) (idx : Nat) (state : State α decls idx) : State α decls decls.size :=
+    if hidx:idx < decls.size then
+      let decl := decls[idx]
+      match hdecl:decl with
+      | .atom a => go decls (idx + 1) (state.addVar a hdecl)
+      | .const b => go decls (idx + 1) (state.addConst b hdecl)
+      | .gate lhs rhs linv rinv => go decls (idx + 1) (state.addGate lhs rhs linv rinv hdecl)
+    else
+      have : idx = decls.size := by
+        have := state.inv2.upper_lt_size
+        omega
+      this ▸ state
+  termination_by decls.size - idx
 
 def State.ofAIG (aig : AIG α) : HashMap α Nat :=
   State.ofAIGAux aig |>.map
@@ -65,12 +134,26 @@ theorem State.ofAIG.Inv1 (aig : AIG α) : ∃ n, State.Inv1 n (State.ofAIG aig) 
   dsimp [ofAIG]
   exact (State.ofAIGAux aig).inv1
 
-/--
-This axiom follows because `State.ofAIG` constructs a map that has every atom inserted.
-However we cannot prove this yet as we don't have enough HashMap theory
--/
-axiom State.ofAIG_find_some {aig : AIG α} : ∀ a ∈ aig, ∃ n, (State.ofAIG aig).find? a = some n
+theorem State.ofAIG.Inv2 (aig : AIG α) : State.Inv2 aig.decls aig.decls.size (State.ofAIG aig) := by
+  have := (State.ofAIGAux aig).inv2
+  simp [State.ofAIG, this]
 
+-- TODO: auxiliary theorem, possibly upstream
+theorem _root_.Array.get_of_mem {a : α} {as : Array α}
+    : a ∈ as → (∃ (i : Fin as.size), as[i] = a) := by
+  intro ha
+  rcases List.get_of_mem ha.val with ⟨i, hi⟩
+  exists i
+
+theorem State.ofAIG_find_some {aig : AIG α} : ∀ a ∈ aig, ∃ n, (State.ofAIG aig).find? a = some n := by
+  intro a ha
+  simp only [mem_def] at ha
+  rcases Array.get_of_mem ha with ⟨⟨i, isLt⟩, hi⟩
+  apply Inv2.property
+  . assumption
+  . exact aig.decls.size
+  . apply ofAIG.Inv2
+  . omega
 
 theorem State.ofAIG_find_unique {aig : AIG α} (a : α) (ha : (State.ofAIG aig).find? a = some n)
     : ∀ a', (State.ofAIG aig).find? a' = some n → a = a' := by
@@ -78,8 +161,10 @@ theorem State.ofAIG_find_unique {aig : AIG α} (a : α) (ha : (State.ofAIG aig).
   rcases State.ofAIG.Inv1 aig with ⟨n, hn⟩
   apply State.Inv1.property <;> assumption
 
+end RelabelNat
+
 def relabelNat (aig : AIG α) : AIG Nat :=
-  let map := State.ofAIG aig
+  let map := RelabelNat.State.ofAIG aig
   aig.relabel fun x =>
     -- The none branch never gets hit, we prove this below
     match map.find? x with
@@ -99,17 +184,17 @@ theorem relabelNat_unsat_iff [Nonempty α] {aig : AIG α} {hidx1} {hidx2}
   . next hcase1 =>
     split at heq
     . next hcase2 =>
-      apply State.ofAIG_find_unique
+      apply RelabelNat.State.ofAIG_find_unique
       . assumption
       . rw [heq]
         assumption
     . next hcase2 =>
       exfalso
-      rcases State.ofAIG_find_some y hy with ⟨n, hn⟩
+      rcases RelabelNat.State.ofAIG_find_some y hy with ⟨n, hn⟩
       simp[hcase2] at hn
   . next hcase =>
     exfalso
-    rcases State.ofAIG_find_some x hx with ⟨n, hn⟩
+    rcases RelabelNat.State.ofAIG_find_some x hx with ⟨n, hn⟩
     simp[hcase] at hn
 
 namespace Entrypoint
